sorted works

merge.dfy
@@ -2,44 +2,78 @@ predicate sorted_seq(a: seq<int>) {
    forall i, j :: 0 <= i < j < |a| ==> a[i] <= a[j]
 }
 
-predicate sorted_until(a: array<int>, until: nat)
-requires until <= a.Length
+predicate sorted_range(a: array<int>, from: nat, until: nat)
+requires from <= until <= a.Length
 reads a {
-    forall i, j :: 0 <= i < j < until ==> a[i] <= a[j]
+    forall i, j :: from <= i < j < until ==> a[i] <= a[j]
 }
 
-predicate permutation_until(a: seq<int>, b: array<int>, until: nat)
-requires until <= b.Length
+predicate permutation_range(a: seq<int>, b: array<int>, from: nat, until: nat)
+requires from <= until <= b.Length
+requires until - from == |a|
 reads b {
-    until == |a| && forall i :: 0 <= i < until ==> b[i] in a
+    var bs := b[from .. until];
+    forall i :: from <= i < |bs| ==> b[i] in a &&
+    forall i :: from <= i < |a| ==> a[i] in bs
 }
 
 predicate sorted(a: array<int>) reads a {
-    forall i, j :: 0 <= i < j < a.Length ==> a[i] <= a[j]
+  sorted_range(a, 0, a.Length)
 }
 
-predicate permutation(a: seq<int>, b: array<int>) reads b {
-    |a| == b.Length && forall i :: 0 <= i < b.Length ==> b[i] in a
+predicate permutation(a: seq<int>, b: array<int>)
+requires |a| == b.Length
+reads b {
+  permutation_range(a, b, 0, b.Length)
+}
+
+method tester()  {
+  var a : seq<int> := [1, 2, 3, 4][..];
+  assert(|a[..0]| == 0);
+}
+
+method copy(a: seq<int>, c: array<int>, at: nat)
+requires at <= c.Length
+requires |a| == c.Length - at
+ensures forall i :: 0 <= i < |a| ==> c[at + i] == a[i]
+modifies c {
+  var i := 0;
+  while (i < |a|)
+  decreases |a| - i
+  invariant 0 <= i <= |a|
+  invariant forall j :: 0 <= j < i ==> c[at + j] == a[j]
+  {
+    c[at + i] := a[i];
+    i := i + 1;
+  }
 }
 
 method merge(a1: seq<int>, a2: seq<int>) returns (res:array<int>)
     requires sorted_seq(a1)
     requires sorted_seq(a2)
     ensures sorted(res)
+    ensures res.Length == |a1| + |a2|
     ensures permutation(a1 + a2, res) {
   if(|a1| == 0 && |a2| == 0) {
     res := new int[0];
     return;
-  } else if (|a1| == 0) {
+  } else if (|a1| == 0) { // res := a2
     res := new int[|a2|];
-    forall i | 0 <= i < |a2| { res[i] := a2[i]; }
+    copy(a2, res, 0);
+    assert(forall i :: 0 <= i < |a2| ==> res[i] == a2[i]);
+    assert(permutation(a2, res));
+    assert(sorted(res));
     return;
-  } else if (|a2| == 0) {
+  } else if (|a2| == 0) { // res := a1
     res := new int[|a1|];
-    forall i | 0 <= i < |a1| { res[i] := a1[i]; }
+    copy(a1, res, 0);
+    assert(forall i :: 0 <= i < |a1| ==> res[i] == a1[i]);
+    assert(permutation(a1, res));
+    assert(sorted(res));
     return;
   }
-  // Now both combined
+
+  // |a1| > 0 && |a2| > 0
   res := new int[|a1| + |a2|];
   var l := 0;
   var r := 0;
@@ -50,12 +84,14 @@ method merge(a1: seq<int>, a2: seq<int>) returns (res:array<int>)
   invariant 0 <= l <= |a1|
   invariant 0 <= r <= |a2|
   invariant i == l + r
-  invariant sorted_until(res, i)
-  invariant permutation_until(a1[..l] + a2[..r], res, i) {
-      assert(forall j:: 0 <= j < i ==> sorted_until(res, j));
-      if(a1[l] < a2[r]) {
+  invariant sorted_range(res, 0, i)
+  invariant forall p, q :: 0 <= p < i && l <= q < |a1| ==> res[p] <= a1[q]
+  invariant forall p, q :: 0 <= p < i && r <= q < |a2| ==> res[p] <= a2[q]
+  invariant permutation_range(a1[..l] + a2[..r], res, 0, i) {
+      if(a1[l] <= a2[r]) {
         res[i] := a1[l];
         l := l + 1;
+        assert(permutation_range(a1[..l] + a2[..r], res, 0, i));
       } else {
         res[i] := a2[r];
         r := r + 1;
@@ -65,14 +101,21 @@ method merge(a1: seq<int>, a2: seq<int>) returns (res:array<int>)
 
   // one of the two is true
   assert(l == |a1| || r == |a2|);
-  assert(i == l + r);
 
   if(l == |a1|) {
-    forall j | r <= j < |a2| { res[l+j] := a2[j]; }
+    var ra2 := a2[r..];
+    copy(ra2, res, i);
+    assert(i == |a1| + r);
+    assert(res.Length == |a1| + |a2|);
+    assert(forall j :: 0 <= j < |ra2| ==> res[i + j] == ra2[j]);
+    assert(forall j :: r <= j < |a2| ==> res[i+j] == a2[j]);
+    assert(sorted_seq(ra2));
+    assert(sorted(res));
     return;
-  }
-  else if(r == |a2|) {
-    forall j | l <= j < |a1| { res[r+j] := a1[j]; }
+  } else if(r == |a2|) {
+    assert(i == l + |a2|);
+    assert(res.Length == |a1| + |a2|);
+    copy(a1[l..], res, i);
     return;
   }
 }
